Halfway through updating kvnode_atomic.

atomics/verif_kvnode_atomic.v
@@ -21,17 +21,20 @@ Opaque upto.
 
 Existing Instances map_PCM fmap_order.
 
-Print ghost_master.
+Definition ghost_log := ghost_master (ORD := @fmap_order nat Z).
+Definition ghost_lsnap := ghost_snap (ORD := @fmap_order nat Z).
+Definition ghost_version := ghost_master (ORD := max_order).
+Definition ghost_vsnap := ghost_snap (ORD := max_order).
 
 Definition node_entry sh v vs locs lg i := EX v' : nat, EX log : nat -> option Z, EX d : Z,
   !!(repable_signed d /\ (if Nat.even v then v' = v /\ d = Znth i vs else (v' >= v - 1)%nat) /\ log_latest log v' d) &&
-  ghost_master(ORD := fmap_order) sh log (Znth i lg) * data_at sh tint (vint d) (Znth i locs).
+  ghost_log sh log (Znth i lg) * data_at sh tint (vint d) (Znth i locs).
 
 Existing Instances nat_PCM max_order.
 
 Definition node_state sh v vs version locs g lg := !!(repable_signed (Z.of_nat v) /\
     Forall repable_signed vs /\ Zlength vs = Zlength locs /\ Zlength lg = Zlength locs) &&
-  ghost_master(ORD := max_order) sh v g * data_at sh tint (vint (Z.of_nat v)) version *
+  ghost_version sh v g * data_at sh tint (vint (Z.of_nat v)) version *
   fold_right sepcon emp (map (node_entry sh v vs locs lg) (upto (length locs))).
 
 Definition node_inv v vs version locs g lg := EX v' : nat, !!(Nat.even v = true /\ (v' = v \/ v' = v + 1)%nat) &&
@@ -116,125 +119,170 @@ Proof.
   intros; apply Z.land_ones with (n := 1); omega.
 Qed.
 
-Lemma singleton_snap : forall (x : Z -> option Z) p v1 v2, x v1 = Some v2 ->
-  view_shift (ghost_snap x p) (ghost_snap (singleton v1 v2) p).
+Lemma singleton_snap : forall x p v1 v2, x v1 = Some v2 ->
+  ghost_lsnap x p |-- |==> ghost_lsnap (singleton v1 v2) p.
 Proof.
   intros.
   apply ghost_snap_forget.
   unfold singleton; intros ??; if_tac; intro X; inv X; auto.
 Qed.
 
+Lemma even_inj : forall n, Z.even (Z.of_nat n) = Nat.even n.
+Proof.
+  induction n; auto.
+  rewrite Nat2Z.inj_succ, Z.even_succ, Nat.even_succ.
+  rewrite <- Z.negb_even, <- Nat.negb_even, IHn; reflexivity.
+Qed.
+
 Lemma body_read : semax_body Vprog Gprog f_read read_spec.
 Proof.
   start_atomic_function.
   destruct x as ((((((((n, out), sh), version), locs), g), lg), v0), vs0); Intros.
-  destruct H as (HP & HQ).
-  eapply semax_loop; [|forward; unfold loop2_ret_assert; apply ENTAIL_refl].
+  unfold atomic_shift; Intros P.
+  set (AS := _ -* _).
+  forward_loop (PROP () LOCAL (temp _n n; temp _out out)
+    SEP (|> P; AS && cored; data_at sh tnode (version, locs) n;
+    data_at_ Tsh (tarray tint 8) out)).
+  { entailer!. }
   repeat forward.
-  forward_call (version, P, II, lI,
-    fun sh v' => !!(sh = gsh2) && EX v : Z, EX vs : _, !!(Z.even v = true /\ Forall repable_signed vs /\
-      Zlength vs = Zlength locs /\ Zlength lg = Zlength locs /\ (v' = v \/ v' = v + 1)) && ghost (gsh2, v') g *
-      fold_right sepcon emp (map (node_entry gsh2 v' vs locs lg) (upto (length locs))) * R (v, vs),
-      fun v : Z => P * ghost_snap v g).
-  { split.
-    + intros.
-      etransitivity; [apply HP|].
-      apply derives_view_shift.
-      Intro x; destruct x as (v, vs).
+  replace_SEP 1 ((AS && cored) * (AS && cored)) by (go_lower; apply cored_dup).
+  forward_call (version, AS && cored * |> P, Full_set iname, Empty_set iname,
+    fun sh v' => !!(sh = gsh2) && EX v : nat, EX vs : _, !!(Nat.even v = true /\ Forall repable_signed vs /\
+      Zlength vs = Zlength locs /\ Zlength lg = Zlength locs /\ (v' = Z.of_nat v \/ v' = Z.of_nat v + 1)) && ghost_version gsh2 (Z.to_nat v') g *
+      fold_right sepcon emp (map (node_entry gsh2 (Z.to_nat v') vs locs lg) (upto (length locs))) *
+      (node_inv v vs version locs g lg -* |={Empty_set iname,Full_set iname}=> |> P),
+      fun v : Z => |> P * ghost_vsnap (Z.to_nat v) g, inv_names).
+  { cancel.
+    rewrite <- emp_sepcon at 1.
+    apply sepcon_derives; [|cancel].
+    rewrite <- emp_sepcon at 1; apply sepcon_derives.
+    + rewrite <- wand_sepcon_adjoint, emp_sepcon.
+      unfold AS.
+      rewrite sepcon_comm.
+      eapply derives_trans; [apply sepcon_derives, andp_left1; apply derives_refl|].
+      eapply derives_trans; [apply modus_ponens_wand | apply fupd_mono].
+      Intros x; destruct x as (v, vs).
+      eapply derives_trans; [apply sepcon_derives, andp_left1; apply derives_refl|].
       unfold node_inv, node_state; Intro v'.
-      Exists gsh2 v' v vs; entailer!.
-    + intros.
-      rewrite <- sepcon_assoc; etransitivity; [|apply view_shift_sepcon1, HP].
-      view_shift_intro v2; view_shift_intro vs; view_shift_intros.
+      Exists gsh2 (Z.of_nat v') v vs; entailer!.
+      rewrite Nat2Z.id; entailer!.
+    + apply allp_right; intro sh1.
+      apply allp_right; intro v1.
+      rewrite <- wand_sepcon_adjoint, emp_sepcon.
+      Intros v2 vs.
       rewrite sepcon_comm, !sepcon_assoc.
-      etransitivity; [apply view_shift_sepcon1, make_snap|].
-      apply derives_view_shift.
-      Exists (v2, vs); unfold node_inv, node_state; Exists v; entailer!. }
+      eapply derives_trans; [apply sepcon_derives, derives_refl; apply make_snap|].
+      eapply derives_trans; [apply bupd_frame_r|].
+      apply fupd_bupd, bupd_mono.
+      eapply derives_trans, fupd_frame_r.
+      rewrite !sepcon_assoc, sepcon_comm; apply sepcon_derives; [|apply derives_refl].
+      rewrite <- !sepcon_assoc, sepcon_comm, <- !sepcon_assoc.
+      apply modus_ponens_wand'.
+      unfold node_inv, node_state.
+      Exists (Z.to_nat v1); entailer!.
+      { destruct H9; subst; try rep_omega.
+        rewrite Z2Nat.inj_add; try omega.
+        rewrite Nat2Z.id; simpl; omega. }
+      rewrite Z2Nat.id by omega.
+      rewrite sepcon_comm; apply derives_refl. }
   Intros v1.
-  match goal with |-semax _ (PROP () (LOCALx ?Q (SEPx ?R))) _ _ =>
-    forward_if (PROP (Z.testbit v1 0 = false) (LOCALx Q (SEPx R))) end.
-  { eapply semax_pre; [|apply semax_continue].
-    unfold POSTCONDITION, abbreviate, overridePost.
-    destruct (eq_dec EK_continue EK_normal); [discriminate|].
-    unfold loop1_ret_assert.
-    entailer!.
-    admit. (* drop snap *) }
+  forward_if (Z.testbit v1 0 = false).
+  { viewshift_SEP 1 emp.
+    { go_lower.
+      apply own_dealloc. }
+    forward.
+    entailer!. }
   { forward.
     entailer!.
+    rewrite Z.bit0_odd.
     unfold Int.one in *; rewrite and_repr, land_1, Zmod_odd in *.
     destruct (Z.odd v1); auto; discriminate. }
   Intros.
-  forward_for_simple_bound 8 (EX i : Z, EX vals : list Z, PROP (Zlength vals = i)
+  forward_for_simple_bound 8 (@exp (environ -> mpred) _ Z (fun i => @exp (environ -> mpred) _ (list Z) (fun vals => PROP (Zlength vals = i)
     LOCAL (temp _snap (vint v1); temp _ver version; temp _n n; temp _out out)
-    SEP (fold_right sepcon emp (map (fun p => invariant (II p)) lI);
-         P; ghost_snap v1 g; @data_at CompSpecs sh tnode (version, locs) n;
+    SEP (|> P; ghost_vsnap (Z.to_nat v1) g; AS && cored; @data_at CompSpecs sh tnode (version, locs) n;
          data_at Tsh (tarray tint 8) (map (fun x => vint x) vals ++ repeat Vundef (Z.to_nat (8 - i))) out;
-         EX vers : list (Z * Z), !!(Zlength vers = i /\
-           Forall (fun '(v, v') => v1 <= v /\ if Z.even v then v' = v else True) vers) &&
-           fold_right sepcon emp (map (fun i => ghost_snap (fst (Znth i vers (0, 0))) g *
-             ghost_snap (singleton (snd (Znth i vers (0, 0))) (Znth i vals 0)) (Znth i lg Vundef))
-             (sublist 0 i (upto 8))))).
-  { Exists (@nil Z) (@nil (Z * Z)); rewrite !sepcon_map; entailer!. }
+         EX vers : list (nat * nat), !!(Zlength vers = i /\
+           Forall (fun '(v, v') => Z.to_nat v1 <= v /\ if Nat.even v then v' = v else True)%nat vers) &&
+           fold_right sepcon emp (map (fun i => ghost_snap (fst (Znth i vers)) g *
+             ghost_lsnap (singleton (snd (Znth i vers)) (Znth i vals)) (Znth i lg))
+             (sublist 0 i (upto 8))))))).
+  { Exists (@nil Z) (@nil (nat * nat)); rewrite !sepcon_map; entailer!.
+    apply data_at__data_at; auto. }
   - Intros vers; rewrite !sepcon_map; Intros.
     forward.
     { entailer!.
       apply Forall_Znth; [omega|].
       eapply Forall_impl; [|eauto]; auto. }
-    forward_call (Znth i locs Vundef, P * ghost_snap v1 g,
-      II, lI,
-      fun sh v => !!(sh = gsh2) && EX ver : Z, EX vs : _, EX ver' : Z, EX v'' : _, EX log : _,
-        !!(repable_signed ver' /\ Z.even ver = true /\ Forall repable_signed vs /\ Zlength vs = Zlength locs /\
-           Zlength lg = Zlength locs /\ (ver' = ver \/ ver' = ver + 1) /\
-           (if Z.even ver' then v'' = ver' /\ v = Znth i vs 0 else v'' >= ver' - 1) /\ log_latest log v'' v) &&
-           ghost (gsh2, ver') g * data_at gsh2 tint (vint ver') version * ghost (gsh2, log) (Znth i lg Vundef) *
+    replace_SEP 2 ((AS && cored) * (AS && cored)) by (go_lower; apply cored_dup).
+    forward_call (Znth i locs, AS && cored * |> P * ghost_vsnap (Z.to_nat v1) g,
+      Full_set iname, Empty_set iname,
+      fun sh v => !!(sh = gsh2) && EX ver : nat, EX vs : _, EX ver' : nat, EX v'' : nat, EX log : _,
+        !!(repable_signed (Z.of_nat ver') /\ Nat.even ver = true /\ Forall repable_signed vs /\ Zlength vs = Zlength locs /\
+           Zlength lg = Zlength locs /\ (ver' = ver \/ ver' = ver + 1)%nat /\
+           (if Nat.even ver' then v'' = ver' /\ v = Znth i vs else v'' >= ver' - 1)%nat /\ log_latest log v'' v) &&
+           ghost_version gsh2 ver' g * data_at gsh2 tint (vint (Z.of_nat ver')) version * ghost_log gsh2 log (Znth i lg) *
            fold_right sepcon emp (upd_Znth i (map (node_entry gsh2 ver' vs locs lg) (upto (length locs))) emp) *
-        R (ver, vs) * ghost_snap v1 g,
-      fun v : Z => P * EX vi : Z, EX v'' : Z, !!(v1 <= vi /\ if Z.even vi then v'' = vi else True) &&
-        ghost_snap v1 g * ghost_snap vi g * ghost_snap (singleton v'' v) (Znth i lg Vundef)).
-(* A common case is to do no view shifts in the first part. In this case, maybe we can provide a magic-wand
-   mpred for P', and prove the magic-wand equivalence separately using wand_sepcon_adjoint. *)
-     { split.
-      + intros.
-        rewrite <- !sepcon_assoc; etransitivity; [apply view_shift_sepcon1, HP|].
-        apply derives_view_shift.
-        Intro s; destruct s as (v, vs).
+        (node_inv ver vs version locs g lg -* |={Empty_set iname,Full_set iname}=> |> P) * ghost_vsnap (Z.to_nat v1) g,
+      fun v : Z => |> P * EX vi : nat, EX v'' : nat, !!(Z.to_nat v1 <= vi /\ if Nat.even vi then v'' = vi else True)%nat &&
+        ghost_vsnap (Z.to_nat v1) g * ghost_vsnap vi g * ghost_lsnap (singleton v'' v) (Znth i lg), inv_names).
+     { cancel.
+      rewrite <- emp_sepcon at 1.
+      apply sepcon_derives; [|cancel].
+      rewrite <- emp_sepcon at 1; apply sepcon_derives.
+      + rewrite <- wand_sepcon_adjoint, emp_sepcon.
+        rewrite (sepcon_comm _ (|> P)).
+        eapply derives_trans; [apply sepcon_derives, derives_refl; apply sepcon_derives, andp_left1; apply derives_refl|].
+        eapply derives_trans; [apply sepcon_derives, derives_refl; apply modus_ponens_wand|].
+        eapply derives_trans; [apply fupd_frame_r | apply fupd_mono].
+        Intros x; destruct x as (v, vs).
+        eapply derives_trans; [apply sepcon_derives, derives_refl; apply sepcon_derives, andp_left1; apply derives_refl|].
         unfold node_inv, node_state; Intros ver'.
         rewrite extract_nth_sepcon with (i := i)
           by (rewrite Zlength_map, Zlength_upto, <- Zlength_correct; omega).
         erewrite Znth_map, Znth_upto by (rewrite ?Zlength_upto, <- Zlength_correct; auto; omega).
         unfold node_entry; Intros v'' log d.
         Exists gsh2 d v vs ver' v'' log; entailer!.
-      + intros.
-        rewrite <- sepcon_assoc; etransitivity; [|apply view_shift_sepcon1, HP].
-        view_shift_intro ver; view_shift_intro vs; view_shift_intro ver'; view_shift_intro v'';
-          view_shift_intro log; view_shift_intros.
-        rewrite sepcon_comm, !sepcon_assoc.
-        etransitivity; [apply view_shift_sepcon1, make_snap|].
-        rewrite <- !sepcon_assoc, (sepcon_comm _ (ghost _ (Znth i lg Vundef))), !sepcon_assoc.
-        etransitivity; [apply view_shift_sepcon1, make_snap|].
-        rewrite sepcon_assoc; etransitivity; [apply view_shift_sepcon1|].
+      + apply allp_right; intro sh1.
+        apply allp_right; intro d1.
+        rewrite <- wand_sepcon_adjoint, emp_sepcon.
+        Intros ver vs ver' v'' log.
+        unfold ghost_version; sep_apply make_snap.
+        eapply derives_trans; [apply bupd_frame_r|].
+        apply fupd_bupd, bupd_mono.
+        unfold ghost_log; sep_apply (make_snap(ORD := @fmap_order nat Z)).
+        eapply derives_trans; [apply bupd_frame_r|].
+        apply fupd_bupd, bupd_mono.
+        fold (ghost_lsnap log (Znth i lg)).
+        rewrite sepcon_assoc; eapply derives_trans; [apply sepcon_derives, derives_refl|].
         { match goal with H : log_latest _ _ _ |- _ => destruct H end.
           apply singleton_snap; eauto. }
-        apply derives_view_shift.
-        assert_PROP (v1 <= ver').
-        { rewrite <- !sepcon_assoc, (sepcon_comm _ (ghost _ g)), (sepcon_comm _ (ghost_snap v1 g)).
-          rewrite <- !sepcon_assoc, snap_master_join by auto; entailer!. }
-        Exists (ver, vs) ver' v''; unfold node_inv, node_state; Exists ver'; entailer!.
-        { if_tac; tauto. }
-        rewrite extract_nth_sepcon with (i := Zlength x)(l := map _ _)
+        eapply derives_trans; [apply bupd_frame_r|].
+        apply fupd_bupd, bupd_mono.
+        eapply derives_trans, fupd_frame_r.
+        assert_PROP (Z.to_nat v1 <= ver')%nat.
+        { unfold ghost_vsnap; sep_apply (snap_master_join (Z.to_nat v1)); auto; entailer!. }
+        Exists ver' v''; entailer!.
+        { simple_if_tac; tauto. }
+        rewrite (sepcon_comm _ (ghost_snap _ g)), !sepcon_assoc, sepcon_comm; apply sepcon_derives, derives_refl.
+        rewrite <- !sepcon_assoc; apply modus_ponens_wand'.
+         unfold node_inv, node_state; Exists ver'; entailer!.
+        rewrite extract_nth_sepcon with (i := Zlength vals)(l := map _ _)
           by (rewrite Zlength_map, Zlength_upto, <- Zlength_correct; omega).
         erewrite Znth_map, Znth_upto by (rewrite ?Zlength_upto, <- Zlength_correct; omega).
-        unfold node_entry; Exists v'' log v; unfold share; entailer!. }
+        unfold node_entry; Exists v'' log d1; unfold share; entailer!.
+        rewrite sepcon_comm; apply derives_refl. }
       Intros vali vi v''.
       forward.
-      Exists (x ++ [vali]) (vers ++ [(vi, v'')]); rewrite !Zlength_app, !Zlength_cons, !Zlength_nil.
+      Exists (vals ++ [vali]) (vers ++ [(vi, v'')]); rewrite !Zlength_app, !Zlength_cons, !Zlength_nil.
       rewrite upd_init, map_app, <- app_assoc, !sepcon_map by (rewrite ?Zlength_map; omega); entailer!.
       { rewrite Forall_app; repeat constructor; auto. }
-      rewrite sublist_split with (mid := Zlength x)(hi := Zlength x + 1) by (rewrite ?Zlength_upto; simpl; omega).
+      rewrite sublist_split with (mid := Zlength vals)(hi := Zlength vals + 1) by (rewrite ?Zlength_upto; simpl; omega).
       erewrite sublist_len_1, Znth_upto by (rewrite ?Zlength_upto; simpl; omega).
       rewrite !map_app, !sepcon_app; simpl.
       rewrite !app_Znth2 by omega.
-      replace (Zlength vers) with (Zlength x); rewrite Zminus_diag, !Znth_0_cons; simpl; cancel.
+      replace (Zlength vers) with (Zlength vals); rewrite Zminus_diag, !Znth_0_cons; simpl; cancel.
+      rewrite (sepcon_comm _ (ghost_snap _ _)), !sepcon_assoc; apply sepcon_derives; [apply derives_refl|].
       rewrite <- !sepcon_map; apply sepcon_list_derives; rewrite !Zlength_map; auto.
       intros ? Hi; erewrite !Znth_map by auto.
       rewrite Zlength_sublist in Hi by (rewrite ?Zlength_upto; simpl; omega).
@@ -243,112 +291,137 @@ Proof.
   - Intros vals vers.
     rewrite app_nil_r, sublist_same by auto; simpl.
     rewrite Z.bit0_odd, Zodd_even_bool in *; destruct (Z.even v1) eqn: Heven; try discriminate.
-    forward_call (version, P * ghost_snap v1 g * fold_right sepcon emp (map (fun i =>
-      ghost_snap (fst (Znth i vers (0, 0))) g *
-      ghost_snap (singleton (snd (Znth i vers (0, 0))) (Znth i vals 0)) (Znth i lg Vundef)) (upto 8)), II, lI,
-      fun sh v' => !!(sh = gsh2) && EX v : Z, EX vs : _, !!(Z.even v = true /\ Forall repable_signed vs /\
-        Zlength vs = Zlength locs /\ Zlength lg = Zlength locs /\ (v' = v \/ v' = v + 1)) &&
-        ghost (gsh2, v') g * fold_right sepcon emp (map (node_entry gsh2 v' vs locs lg) (upto (length locs))) *
-        R (v, vs) * ghost_snap v1 g * fold_right sepcon emp (map (fun i => ghost_snap (fst (Znth i vers (0, 0))) g *
-          ghost_snap (singleton (snd (Znth i vers (0, 0))) (Znth i vals 0)) (Znth i lg Vundef)) (upto 8)),
-      fun v : Z => (if eq_dec v v1 then Q (v, vals) tt else P) *
-        (!!(if eq_dec v v1 then Forall (fun '(vi, v') => vi = v1 /\ v' = v1) vers else True) &&
-        ghost_snap v g * fold_right sepcon emp (map (fun i => ghost_snap (fst (Znth i vers (0, 0))) g *
-          ghost_snap (singleton (snd (Znth i vers (0, 0))) (Znth i vals 0)) (Znth i lg Vundef)) (upto 8)))).
-    { split.
-      + intros.
-        rewrite <- !sepcon_assoc, sepcon_assoc; etransitivity; [apply view_shift_sepcon; [apply HP | reflexivity]|].
-        apply derives_view_shift.
-        Intro x; destruct x as (v, vs).
+    replace_SEP 2 ((AS && cored) * (AS && cored)) by (go_lower; apply cored_dup).
+    forward_call (version, AS && cored * |> P * ghost_vsnap (Z.to_nat v1) g * fold_right sepcon emp (map (fun i =>
+      ghost_vsnap (fst (Znth i vers)) g * ghost_lsnap (singleton (snd (Znth i vers)) (Znth i vals)) (Znth i lg)) (upto 8)) *
+      data_at sh tnode (version, locs) n * data_at Tsh (tarray tint 8) (map (fun x : Z => vint x) vals) out,
+      Full_set iname, Empty_set iname,
+      fun sh' v' => !!(sh' = gsh2) && EX v : nat, EX vs : _, !!(Nat.even v = true /\ Forall repable_signed vs /\
+        Zlength vs = Zlength locs /\ Zlength lg = Zlength locs /\ (v' = Z.of_nat v \/ v' = Z.of_nat v + 1)) &&
+        ghost_version gsh2 (Z.to_nat v') g * fold_right sepcon emp (map (node_entry gsh2 (Z.to_nat v') vs locs lg) (upto (length locs))) *
+        data_at sh tnode (version, locs) n * data_at Tsh (tarray tint 8) (map (fun x : Z => vint x) vals) out *
+        ((node_inv v vs version locs g lg -* |={Empty_set iname,Full_set iname}=> |> P) &&
+         (ALL y : unit, (data_at sh tnode (version, locs) n *
+                data_at Tsh (tarray tint 8) (map (fun x0 : Z => vint x0) vs) out *
+                node_inv v vs version locs g lg) -* |={ Empty_set iname, Full_set iname }=> Q y)) * ghost_vsnap (Z.to_nat v1) g * fold_right sepcon emp (map (fun i => ghost_vsnap (fst (Znth i vers)) g *
+          ghost_lsnap (singleton (snd (Znth i vers)) (Znth i vals)) (Znth i lg)) (upto 8)),
+      fun v : Z => (if eq_dec v v1 then Q tt else |> P *
+          data_at sh tnode (version, locs) n * data_at Tsh (tarray tint 8) (map (fun x : Z => vint x) vals) out) *
+        (!!(if eq_dec v v1 then Forall (fun '(vi, v') => vi = Z.to_nat v1 /\ v' = Z.to_nat v1) vers else True) &&
+        ghost_vsnap (Z.to_nat v) g * fold_right sepcon emp (map (fun i => ghost_snap (fst (Znth i vers)) g *
+          ghost_lsnap (singleton (snd (Znth i vers)) (Znth i vals)) (Znth i lg)) (upto 8))), inv_names).
+    { unfold ghost_vsnap; cancel.
+      rewrite <- emp_sepcon at 1.
+      apply sepcon_derives; [|cancel].
+      rewrite <- emp_sepcon at 1; apply sepcon_derives.
+      + rewrite <- wand_sepcon_adjoint, emp_sepcon.
+        rewrite (sepcon_comm _ (|> P)), 3sepcon_assoc.
+        eapply derives_trans; [apply sepcon_derives, derives_refl; apply sepcon_derives, andp_left1; apply derives_refl|].
+        eapply derives_trans; [apply sepcon_derives, derives_refl; apply modus_ponens_wand|].
+        eapply derives_trans; [apply fupd_frame_r | apply fupd_mono].
+        Intros x; destruct x as (v, vs).
         unfold node_inv, node_state; Intro v'.
-        Exists gsh2 v' v vs; entailer!.
-      + intros.
+        Exists gsh2 (Z.of_nat v') v vs; entailer!.
+        rewrite Nat2Z.id; auto.
+      + apply allp_right; intro sh0.
+        apply allp_right; intro v.
+        rewrite <- wand_sepcon_adjoint, emp_sepcon.
         destruct (eq_dec v v1).
-        * view_shift_intro ver; view_shift_intro vs; view_shift_intros; subst.
-          match goal with H : _ \/ _ |- _ => destruct H; subst;
-            [|match goal with H : Z.even (ver + 1) = true |- _ => rewrite Z.even_add in H;
-              replace (Z.even ver) with true in H; discriminate end] end.
-          apply view_shift_assert with (PP := Forall (fun '(vi, v') => vi = ver /\ v' = ver) vers).
-          { rewrite Forall_forall_Znth with (d := (0, 0)), prop_forall; apply allp_right; intro i.
+        * Intros ver vs; subst.
+          match goal with H : _ \/ _ |- _ => destruct H; subst; [|match goal with H : Z.even (Z.of_nat ver + 1) = true |- _ => rewrite Z.even_add, even_inj in H;
+              replace (Nat.even ver) with true in H; discriminate end] end.
+          rewrite Nat2Z.id in *.
+          assert_PROP (Forall (fun '(vi, v') => vi = ver /\ v' = ver) vers) as Hvers.
+          { rewrite Forall_forall_Znth, prop_forall; apply allp_right; intro i.
             rewrite prop_forall; apply allp_right; intro.
-            match goal with H : Forall _ vers |- _ => apply Forall_Znth with (i0 := i)(d := (0, 0)) in H; auto end.
+            match goal with H : Forall _ vers |- _ => apply Forall_Znth with (i0 := i) in H; auto end.
             rewrite extract_nth_sepcon with (i := i)(l := map _ (upto 8))
               by (rewrite Zlength_map, Zlength_upto; simpl; omega).
             erewrite Znth_map, Znth_upto by (rewrite ?Zlength_upto; simpl; omega).
-            rewrite <- !sepcon_assoc, (sepcon_comm _ (ghost _ g)), (sepcon_comm _ (ghost_snap (fst _) g)).
-            rewrite <- !sepcon_assoc, snap_master_join by auto.
-            Intros; apply prop_right; destruct (Znth i vers (0, 0)); simpl in *.
-            assert (z = ver) by omega; subst.
-            destruct (Z.even ver); try discriminate; tauto. }
-          intro Hvers.
-          etransitivity; [|etransitivity; [apply view_shift_sepcon with (Q' :=
-            ghost_snap ver g * fold_right sepcon emp (map (fun i => ghost_snap (fst (Znth i vers (0, 0))) g *
-              ghost_snap (singleton (snd (Znth i vers (0, 0))) (Znth i vals 0)) (Znth i lg Vundef)) (upto 8)));
-            [apply (HQ (ver, vals) tt) | reflexivity] | apply derives_view_shift; entailer!]].
-          apply derives_view_shift.
+            rewrite <- !sepcon_assoc, (sepcon_comm _ (ghost_version _ _ g)), (sepcon_comm _ (ghost_vsnap (fst (Znth i vers)) g)).
+            unfold ghost_vsnap, ghost_version; rewrite <- !sepcon_assoc, snap_master_join by auto.
+            Intros; apply prop_right; destruct (Znth i vers) as (z, ?); simpl in *.
+            assert (z = ver) by rep_omega; subst.
+            destruct (Nat.even ver); try discriminate; tauto. }
+          rewrite prop_true_andp by auto.
           assert_PROP (vs = vals).
-          { assert_PROP (forall i, 0 <= i < Zlength vs -> Znth i vs 0 = Znth i vals 0);
+          { assert_PROP (forall i, 0 <= i < Zlength vs -> Znth i vs = Znth i vals);
               [|eapply prop_right, list_Znth_eq'; auto; omega].
             rewrite prop_forall; apply allp_right; intro i.
             rewrite prop_forall; apply allp_right; intro.
-            apply Forall_Znth with (i0 := i)(d := (0, 0)) in Hvers; [|omega].
+            apply Forall_Znth with (i0 := i) in Hvers; [|omega].
             rewrite extract_nth_sepcon with (i := i)
               by (rewrite Zlength_map, Zlength_upto, <- Zlength_correct; omega).
             rewrite extract_nth_sepcon with (i := i)(l := map _ _)
               by (rewrite Zlength_map, Zlength_upto; simpl; omega).
             erewrite !Znth_map, !Znth_upto by (rewrite ?Zlength_upto, <- ?Zlength_correct; simpl; omega).
             unfold node_entry; Intros v' log d.
-            destruct (Z.even ver); try discriminate.
-            destruct (Znth i vers (0, 0)); repeat match goal with H : _ = _ /\ _ = _ |- _ => destruct H end.
-            subst; rewrite <- !sepcon_assoc, (sepcon_comm _ (ghost _ (Znth i lg Vundef))),
-              (sepcon_comm _ (ghost_snap _ (Znth i lg Vundef))).
-            rewrite <- !sepcon_assoc, snap_master_join by auto; simpl; Intros; apply prop_right.
+            destruct (Nat.even ver); try discriminate.
+            destruct (Znth i vers); repeat match goal with H : _ = _ /\ _ = _ |- _ => destruct H end.
+            subst; rewrite <- !sepcon_assoc, (sepcon_comm _ (ghost_log _ _ (Znth i lg))),
+              (sepcon_comm _ (ghost_lsnap _ (Znth i lg))).
+            unfold ghost_log, ghost_lsnap; rewrite <- !sepcon_assoc, snap_master_join by auto; simpl; Intros; apply prop_right.
             unfold singleton in *.
             match goal with H : log_latest _ _ _ |- _ => destruct H end.
             match goal with H : map_incl _ _ |- _ => specialize (H ver); simpl in H; rewrite eq_dec_refl in H;
               specialize (H _ eq_refl); rewrite H in *; congruence end. }
+          rewrite sepcon_assoc; eapply derives_trans, fupd_frame_r; cancel.
+          eapply derives_trans; [apply sepcon_derives, andp_left2, allp_left with tt; apply derives_refl|].
+          apply modus_ponens_wand'.
           subst; unfold node_inv, node_state; Exists ver; entailer!.
-        * rewrite <- !sepcon_assoc, sepcon_assoc; etransitivity; [|apply view_shift_sepcon; [apply HP | reflexivity]].
-          view_shift_intro ver; view_shift_intro vs; view_shift_intros.
-          rewrite <- !sepcon_assoc, (sepcon_comm _ (ghost _ _)), (sepcon_comm _ (ghost_snap _ _)).
-          rewrite <- !sepcon_assoc, snap_master_join by auto.
-          view_shift_intros; rewrite !sepcon_assoc; etransitivity; [apply view_shift_sepcon1, make_snap|].
-          apply derives_view_shift; Exists (ver, vs); unfold node_inv, node_state; Exists v; entailer!. }
+        * Intros ver vs.
+          rewrite <- !sepcon_assoc, (sepcon_comm _ (ghost_version _ _ _)), (sepcon_comm _ (ghost_vsnap _ _)).
+          unfold ghost_version, ghost_vsnap; rewrite <- !sepcon_assoc, snap_master_join by auto.
+          Intros; sep_apply make_snap.
+          eapply derives_trans; [apply bupd_frame_r|].
+          apply fupd_bupd, bupd_mono.
+          rewrite !sepcon_assoc; eapply derives_trans, fupd_frame_r; cancel.
+          rewrite <- !sepcon_assoc; eapply derives_trans; [apply sepcon_derives, andp_left1; apply derives_refl|].
+          apply modus_ponens_wand'.
+          unfold node_inv, node_state; Exists (Z.to_nat v); entailer!.
+          { destruct H14; subst; try rep_omega.
+            rewrite Z2Nat.inj_add, Nat2Z.id; simpl; omega. }
+          unfold ghost_version; rewrite Z2Nat.id by omega; auto. }
     Intros v2.
-    match goal with |-semax _ (PROP () (LOCALx ?Q (SEPx ?R))) _ _ =>
-      forward_if (PROP (v2 <> v1) (LOCALx Q (SEPx R))) end.
+    forward_if (v2 <> v1).
     + subst; rewrite eq_dec_refl in *.
+      viewshift_SEP 1 emp.
+      { go_lower; apply own_dealloc. }
+      viewshift_SEP 2 emp.
+      { go_lower.
+        rewrite sepcon_map.
+        eapply derives_trans; [apply sepcon_derives|].
+        * (* apply own_list_dealloc'. *) admit.
+        * (* apply own_list_dealloc'. *) admit.
+        * rewrite sepcon_emp; apply derives_refl. }
       forward.
-      Exists tt (v1, vals); entailer!.
-      admit. (* drop snaps *)
+      Exists tt; entailer!.
+      admit.
     + forward.
       entailer!.
-    + intros; unfold overridePost.
-      destruct (eq_dec ek EK_normal); [subst | apply ENTAIL_refl].
-      unfold POSTCONDITION, abbreviate, loop1_ret_assert.
-      Intros; if_tac; [contradiction | entailer!].
+    + Intros; if_tac; [contradiction | entailer!].
       admit. (* drop snaps *)
 Admitted.
 
-Lemma dirty_entry : forall sh v vs locs lg i, Z.even v = true ->
+Lemma dirty_entry : forall sh v vs locs lg i, Nat.even v = true ->
   node_entry sh v vs locs lg i |-- node_entry sh (v + 1) vs locs lg i.
 Proof.
   intros; unfold node_entry.
   Intros v' log d.
   rewrite H in *; match goal with H : _ /\ _ |- _ => destruct H end.
   Exists v log d; entailer!.
-  rewrite Z.even_add, H; simpl; omega.
+  rewrite Nat.even_add, H; simpl; omega.
 Qed.
 
-Lemma clean_entry : forall v vs locs lg i vs', Z.even v = false ->
+Lemma clean_entry : forall v vs locs lg i vs', Nat.even v = false ->
   node_entry gsh1 (v + 1) vs' locs lg i * node_entry gsh2 v vs locs lg i |--
   node_entry gsh1 (v + 1) vs' locs lg i * node_entry gsh2 (v + 1) vs' locs lg i.
 Proof.
   intros; unfold node_entry.
   Intros v1 log1 d1 v2 log2 d2.
-  Exists (v + 1) log1 d1 (v + 1) log1 d1.
+  Exists (v + 1)%nat log1 d1 (v + 1)%nat log1 d1.
   rewrite sepcon_assoc, (sepcon_comm (data_at _ _ _ _)), <- !sepcon_assoc.
-  erewrite master_share_join' by eauto.
+  unfold ghost_log; erewrite master_share_join' by eauto.
   assert_PROP (d1 = d2).
   { rewrite sepcon_assoc, sepcon_comm; apply sepcon_derives_prop.
     unfold data_at, field_at, at_offset; rewrite !data_at_rec_eq; simpl; Intros.
@@ -357,11 +430,11 @@ Proof.
     apply repr_inj_signed; auto; congruence. }
   erewrite <- master_share_join by eauto; entailer!.
   exploit (log_latest_inj log2 v1 d2 v2); eauto; intros (? & ?); subst.
-  rewrite Z.even_add, H in *; simpl in *.
+  rewrite Nat.even_add, H in *; simpl in *.
   match goal with H : _ /\ _ |- _ => destruct H; subst; repeat (split; auto) end.
 Qed.
 
-Corollary clean_entries : forall v vs locs lg vs', Z.even v = false ->
+Corollary clean_entries : forall v vs locs lg vs', Nat.even v = false ->
   fold_right sepcon emp (map (node_entry gsh1 (v + 1) vs' locs lg) (upto 8)) *
   fold_right sepcon emp (map (node_entry gsh2 v vs locs lg) (upto 8)) |--
   fold_right sepcon emp (map (node_entry gsh1 (v + 1) vs' locs lg) (upto 8)) *
